template-coq/theories/Typing.v
@@ -563,7 +563,7 @@ Fixpoint destArity Γ (t : term) :=
 
 Reserved Notation " Σ ;;; Γ |- t : T " (at level 50, Γ, t, T at next level).
 Reserved Notation " Σ ;;; Γ |- t <= u " (at level 50, Γ, t, u at next level).
-
+Reserved Notation " Σ ;;; Γ |- t = u " (at level 50, Γ, t, u at next level).
 (** ** Cumulativity *)
 
 Inductive cumul `{checker_flags} (Σ : global_env_ext) (Γ : context) : term -> term -> Type :=
@@ -578,12 +578,14 @@ where " Σ ;;; Γ |- t <= u " := (cumul Σ Γ t u) : type_scope.
    Defined as cumulativity in both directions.
  *)
 
-Definition conv `{checker_flags} Σ Γ T U : Type :=
-  (Σ ;;; Γ |- T <= U) * (Σ ;;; Γ |- U <= T).
+Inductive conv `{checker_flags} (Σ : global_env_ext) (Γ : context) : term -> term -> Type :=
+ | conv_refl t u : eq_term (global_ext_constraints Σ) t u -> Σ ;;; Γ |- t = u
+ | conv_red_l t u v : red1 Σ.1 Γ t v -> Σ ;;; Γ |- v = u -> Σ ;;; Γ |- t = u
+ | conv_red_r t u v : Σ ;;; Γ |- t = v -> red1 Σ.1 Γ u v -> Σ ;;; Γ |- t = u
 
-Notation " Σ ;;; Γ |- t = u " := (conv Σ Γ t u) (at level 50, Γ, t, u at next level) : type_scope.
+ where " Σ ;;; Γ |- t = u " := (@conv _ Σ Γ t u) : type_scope.
 
-Lemma conv_refl `{checker_flags} : forall Σ Γ t, Σ ;;; Γ |- t = t.
+Lemma conv_refl' `{checker_flags} : forall Σ Γ t, Σ ;;; Γ |- t = t.
   intros. todo "conv_refl".
 Defined.
 
